Latest changes on this branch.

Hybrid_Programs/Verification_Examples/RoboSim.thy
@@ -31,12 +31,261 @@ dataspace robosim =
     TimeScale :: real
   variables
     executing :: bool
+    wait  :: bool
     timer :: real
     t     :: real
 
 context robosim
 begin
 
+abbreviation "T(P) \<equiv> IF \<not> wait THEN P ELSE skip"
+                                       
+definition "TimerEvo \<delta> a \<sigma> B \<equiv> g_dl_ode_frame (t +\<^sub>L timer +\<^sub>L a) (\<sigma>(t  \<leadsto> 1, timer \<leadsto> 1)) (@B \<and> $timer \<le> \<guillemotleft>\<delta>\<guillemotright>)\<^sub>e"
+
+lemma TimerEvo_delta_nmods:
+  assumes "TimerEvo \<delta> a \<sigma> B nmods P"
+  shows "\<^bold>{ P \<^bold>} TimerEvo \<delta> a \<sigma> B \<^bold>{ P \<and> $timer \<le> \<guillemotleft>\<delta>\<guillemotright> \<^bold>}"
+  apply (simp only:hoare_conj_pos, auto)
+  using assms nmods_invariant apply fastforce
+  using TimerEvo_def by (smt (verit, del_insts) SEXP_def fbox_g_orbital_on)
+
+lemma TimerEvo_pos_timer_delta:
+  shows "\<^bold>{ P \<^bold>} TimerEvo \<delta> a \<sigma> B \<^bold>{ $timer \<le> \<guillemotleft>\<delta>\<guillemotright> \<^bold>}"
+  using TimerEvo_def
+  by (smt (verit, best) SEXP_def fbox_g_orbital_on predicate1I)
+ 
+definition 
+  "EvolveUntil \<delta> a \<sigma> \<equiv> 
+    T(timer ::= 0 ; wait ::= True ; TimerEvo \<delta> a \<sigma> (True)\<^sup>e ; 
+      (IF timer \<ge> \<guillemotleft>\<delta>\<guillemotright> THEN wait ::= False ELSE skip)
+     )"
+
+thm nmods_Choice
+
+lemma
+  assumes "vwb_lens a" "$t \<sharp> e" "$timer \<sharp> e" "$a \<sharp> e" "$wait \<sharp> e" 
+  shows "EvolveUntil \<delta> a \<sigma> nmods e"
+  using assms
+  apply (simp add: EvolveUntil_def TimerEvo_def)
+  apply (auto intro!: closure)
+     apply (expr_auto)+
+  done
+
+term "[a \<leadsto> b]"
+thm "unrest_expr"
+find_theorems "g_orbital_on"
+term "a\<lbrakk>v/x\<rbrakk>"
+term "( ($wait\<lbrakk>v/a\<rbrakk>)\<^sub>e = ($wait)\<^sub>e)"
+
+lemma "($wait\<lbrakk>1/timer\<rbrakk>)\<^sub>e = ($wait)\<^sub>e"
+  by (expr_auto)
+
+lemma "($wait\<lbrakk>wait/wait\<rbrakk>)\<^sub>e = ($wait)\<^sub>e"
+  by (expr_auto)
+
+lemma "($wait\<lbrakk>False/wait\<rbrakk>)\<^sub>e = (False)\<^sub>e"
+  by expr_auto
+
+lemma lens_indep_no_change:
+  assumes "x \<bowtie> y" 
+  shows "($y\<lbrakk>v/x\<rbrakk>)\<^sub>e = ($y)\<^sub>e"
+  by (simp add: assms lens_indep.lens_put_irr2 subst_app_def subst_id_def subst_upd_def)
+
+lemma lens_indep_no_change'[simp]:
+  assumes "y \<bowtie> x" 
+  shows "get\<^bsub>x\<^esub> ([y \<leadsto> b] d) = get\<^bsub>x\<^esub> d"
+  by (simp add: assms get_subst_upd_indep subst_id_def lens_indep_sym)
+
+(* This is a notion weaker than lens independence, but not sure if it's worth working with it! *)
+lemma 
+  assumes "(\<And>v. ($y\<lbrakk>v/x\<rbrakk>)\<^sub>e = ($y)\<^sub>e)"
+  shows "x \<bowtie> y"
+  apply (rule lens_indepI)
+  defer defer
+  using assms apply expr_auto 
+     apply meson+
+  oops
+
+lemma 
+  assumes "(\<And>v. ($y\<lbrakk>v/x\<rbrakk>)\<^sub>e = ($y)\<^sub>e)"
+  shows "x ##\<^sub>L y"
+  unfolding lens_compat_def
+  unfolding lens_override_def
+  using assms apply auto 
+  apply expr_auto
+  oops
+
+lemma EvolveUntil_not_wait:
+  (* Need assumption that a does not modify wait. Stated below using substitution:
+     essentially, it must be the case that for every possible state v, when
+     a is substituted in $wait by v, then its value doesn't change. *)
+
+  (* I've removed the assumption: (\<And>v. ($wait\<lbrakk>v/a\<rbrakk>)\<^sub>e = ($wait)\<^sub>e) in favour of lens independence,
+     which is stronger, but practically I think nearly always wanted for this result. *)
+  assumes "a \<bowtie> wait"
+  shows "\<^bold>{ \<not> wait \<^bold>} EvolveUntil \<delta> a \<sigma> \<^bold>{ \<not> wait \<longrightarrow> timer = \<guillemotleft>\<delta>\<guillemotright> \<^bold>}"
+  unfolding EvolveUntil_def
+  apply (rule hoare_if_then_else)
+  apply ((simp only:kcomp_assoc)?, rule hoare_floyd_kcomp, simp)
+   apply ((simp only:kcomp_assoc)?, rule hoare_floyd_kcomp, simp, subst_eval)
+   apply (rule hoare_kcomp[where R="($wait \<and> $timer \<le> \<guillemotleft>\<delta>\<guillemotright>)\<^sup>e"])
+    apply (rule hoare_weaken_pre_conj[where P="($wait)\<^sup>e"], simp)
+    apply (rule TimerEvo_delta_nmods)
+  unfolding TimerEvo_def apply (auto intro!:closure; subst_eval)
+  using assms apply simp
+     (* (\<And>v. ?a\<lbrakk>v/?x\<rbrakk> = (?a)\<^sub>e) *)
+    apply wlp_full+
+  done
+
+(* Need a lemma that states: if the rate of change of a variable is
+   the same as another, then they are changed by the same amount.*) 
+
+lemma hoare_T_wait:
+  assumes "\<^bold>{P \<and> \<not> wait\<^bold>} C \<^bold>{Q\<^bold>}" "`(P \<and> wait) \<longrightarrow> Q`"
+  shows "\<^bold>{P\<^bold>} T C \<^bold>{Q\<^bold>}"
+  apply (rule hoare_if_then_else)
+  using assms apply simp
+  by (metis (mono_tags, lifting) SEXP_def assms(2) fbox_skip predicate1I taut_def)
+
+lemma "vwb_lens a \<Longrightarrow> a \<bowtie> t \<Longrightarrow> a \<bowtie> timer \<Longrightarrow> vwb_lens (timer +\<^sub>L t +\<^sub>L a)"
+  by (meson indeps(11) lens_indep_sym plus_pres_lens_indep' plus_vwb_lens vwbs(3) vwbs(4))
+
+thm differentiable_dvar
+
+(* The following is useful when there is an explicit lens composition.
+   FIXME: Move to Framed_Derivatives.thy. *)
+lemma differentiable_cvar_explicit[ldifferentiable]:
+  assumes "vwb_lens X" "vwb_lens x" "X \<bowtie> x"
+  shows "differentiable\<^bsub>x +\<^sub>L X\<^esub> $x within S when G"
+  apply (rule differentiable_cvar)
+  using assms lens_indep_sym plus_vwb_lens vwbs(4) apply blast
+   apply (simp add: assms(1))
+  by (simp add: assms(1) assms(2) assms(3) lens_indep_sym)  
+
+lemma "vwb_lens x \<Longrightarrow> vwb_lens y \<Longrightarrow> x \<bowtie> y \<Longrightarrow> vwb_lens (y +\<^sub>L x)"
+  using lens_indep_sym plus_vwb_lens by blast
+
+(* The following is useful when the lens independence is stated in the opposite
+   way to the lens composition. FIXME: add to Lens_Algebra.thy ? *)
+lemma plus_vwb_lens' [simp]:
+  assumes "vwb_lens x" "vwb_lens y" "y \<bowtie> x"
+  shows "vwb_lens (x +\<^sub>L y)"
+  using assms
+  by (meson lens_indep_sym plus_vwb_lens)
+
+lemma TimerEvo_t_increasing:
+  assumes "vwb_lens a" "t \<bowtie> a" "timer \<bowtie> a"
+  shows "\<^bold>{ \<guillemotleft>t\<^sub>1\<guillemotright> \<le> t \<^bold>} TimerEvo \<delta> a \<sigma> (True)\<^sup>e \<^bold>{ \<guillemotleft>t\<^sub>1\<guillemotright> \<le> t \<^bold>}"
+  unfolding TimerEvo_def (* despite the above dInduct can fail if t \<bowtie> a is swapped by a \<bowtie> t *)
+  using assms by (dInduct)
+ 
+lemma TimerEvo_t_increasing':
+  assumes "vwb_lens a" "t \<bowtie> a" "timer \<bowtie> a"
+  shows "\<^bold>{ \<guillemotleft>t\<^sub>1\<guillemotright> = t \<^bold>} TimerEvo \<delta> a \<sigma> (True)\<^sup>e \<^bold>{ \<guillemotleft>t\<^sub>1\<guillemotright> \<le> t \<^bold>}"
+  using assms TimerEvo_t_increasing 
+  by fastforce
+
+lemma TimerEvo_timer_sum_invariant:
+  assumes "vwb_lens a" "t \<bowtie> a" "timer \<bowtie> a"
+  shows " \<^bold>{ t = \<guillemotleft>t\<^sub>0\<guillemotright> + timer \<^bold>} TimerEvo \<delta> a \<sigma> (True)\<^sup>e \<^bold>{ t = \<guillemotleft>t\<^sub>0\<guillemotright> + timer \<^bold>}"
+  using assms unfolding TimerEvo_def 
+  by (dInduct)
+
+lemma TimerEvo_timer_sum_invariant':
+  assumes "vwb_lens a" "t \<bowtie> a" "timer \<bowtie> a"
+  shows " \<^bold>{ t = \<guillemotleft>t\<^sub>0\<guillemotright> \<and> timer = 0 \<^bold>} TimerEvo \<delta> a \<sigma> (True)\<^sup>e \<^bold>{ t = \<guillemotleft>t\<^sub>0\<guillemotright> + timer \<^bold>}"
+  using assms 
+  apply (hoare_wp_auto)
+  by (smt (verit, best) SEXP_def TimerEvo_timer_sum_invariant fbox_iso predicate1D predicate1I)
+  (* FIXME: There ought to be a better non-SMT proof for the above. *)
+
+lemma hoare_weaken_pre:
+  assumes "`P \<longrightarrow> Q`" and "\<^bold>{Q\<^bold>} G \<^bold>{R\<^bold>}"
+  shows "\<^bold>{P\<^bold>} G \<^bold>{R\<^bold>}"
+  using assms oops
+
+lemma hoare_stengthen_post:
+  assumes "`Q \<longrightarrow> R`" and "\<^bold>{P\<^bold>} G \<^bold>{Q\<^bold>}"
+  shows "\<^bold>{P\<^bold>} G \<^bold>{R\<^bold>}"
+  using assms Diff_Dyn_Logic.strengthen by blast
+
+thm nmods_frame_law
+
+
+
+lemma g_dl_ode_frame_nmods:
+  assumes "a \<bowtie> x" "vwb_lens x"
+  shows "g_dl_ode_frame a \<sigma> B nmods $x"
+  using assms unfolding not_modifies_def apply auto
+  using g_orbital_on_def   
+  by (smt (verit, del_insts) g_orbital_on_eq lens_indep.lens_put_irr2 mem_Collect_eq)
+
+lemma TimerEvo_nmods_lens:
+  assumes "a \<bowtie> x" "timer \<bowtie> x" "t \<bowtie> x" "vwb_lens x"
+  shows "TimerEvo \<delta> a \<sigma> B nmods $x"
+proof -
+  have "(t +\<^sub>L timer +\<^sub>L a) \<bowtie> x"
+    using assms 
+    by force
+  then show ?thesis
+    unfolding TimerEvo_def using assms g_dl_ode_frame_nmods
+    by blast
+qed
+
+lemma EvolveUntil_t_not_wait:
+  (* Need assumption that a does not modify wait. Stated below using substitution:
+     essentially, it must be the case that for every possible state v, when
+     a is substituted in $wait by v, then its value doesn't change. *)
+  assumes "a \<bowtie> wait" "TimerEvo \<delta> a \<sigma> (True)\<^sup>e nmods P" "$wait \<sharp> P" "$timer \<sharp> P" "vwb_lens a" "t \<bowtie> a" "timer \<bowtie> a"
+  shows "\<^bold>{ P \<and> t = \<guillemotleft>t\<^sub>0\<guillemotright> \<and> \<not> wait \<^bold>} EvolveUntil \<delta> a \<sigma> \<^bold>{ P \<and> (\<not> wait \<longleftrightarrow> t = \<guillemotleft>t\<^sub>0\<guillemotright> + \<guillemotleft>\<delta>\<guillemotright>) \<and> (wait \<longleftrightarrow> t < \<guillemotleft>t\<^sub>0\<guillemotright> + \<guillemotleft>\<delta>\<guillemotright>)\<^bold>}"
+  unfolding EvolveUntil_def
+   apply (rule hoare_if_then_else)
+    apply ((simp only:kcomp_assoc)?, rule hoare_floyd_kcomp, simp)
+   apply ((simp only:kcomp_assoc)?, rule hoare_floyd_kcomp, simp, subst_eval)
+  defer
+   apply expr_auto
+  apply (rule hoare_kcomp[where R="(P \<and> wait \<and> t = \<guillemotleft>t\<^sub>0\<guillemotright> + timer \<and> timer \<le> \<guillemotleft>\<delta>\<guillemotright> )\<^sup>e"])
+   defer
+   apply (rule hoare_if_then_else)
+  using assms apply (hoare_wp_auto)
+  using assms apply (hoare_wp_auto)
+  apply (rule hoare_weaken_pre_conj[where P="(P \<and> wait \<and> t = \<guillemotleft>t\<^sub>0\<guillemotright> + timer)\<^sup>e"])
+  using assms(3,4) apply expr_auto
+  apply (rule hoare_conj_posI[where a="(P \<and> wait \<and> t = \<guillemotleft>t\<^sub>0\<guillemotright> + timer)\<^sup>e" and b="(timer \<le> \<guillemotleft>\<delta>\<guillemotright>)\<^sup>e"])
+    defer
+    apply (simp add: TimerEvo_pos_timer_delta)
+  apply expr_auto
+  apply (rule nmods_frame_law'', simp add:assms)
+  apply (rule nmods_frame_law'', simp add:assms TimerEvo_nmods_lens)
+  by (simp add:assms TimerEvo_timer_sum_invariant) 
+
+lemma 
+  assumes "a \<bowtie> wait" 
+          "TimerEvo \<delta> a \<sigma> (True)\<^sup>e nmods P" (* Might want to relax this assumption. *)
+          "$wait \<sharp> P" "$timer \<sharp> P" "vwb_lens a" "t \<bowtie> a" "timer \<bowtie> a"
+          "`(P \<and> t = \<guillemotleft>t\<^sub>0\<guillemotright> + \<guillemotleft>\<delta>\<guillemotright>) \<longrightarrow> R`"
+         (* "\<^bold>{ t = \<guillemotleft>t\<^sub>1\<guillemotright> \<^bold>} C \<^bold>{ \<guillemotleft>t\<^sub>1\<guillemotright> \<le> t \<^bold>}" *)
+          "\<^bold>{R\<^bold>} C \<^bold>{R\<^bold>}"
+    (* What we want: 
+        * P is an invariant over EvolveUntil, and so:
+           * it holds at t = t\<^sub>0 and at t = t\<^sub>0 + \<delta>
+        * R is an invariant over C, and so:
+           * it holds at t = t\<^sub>0 + \<delta> as established by EvolveUntil at t = t\<^sub>0 + \<delta>,
+             so perhaps it is sufficient to show that `P \<and> t = t\<^sub>0 + \<delta> \<longrightarrow> R` ?
+    *)
+  shows "\<^bold>{P \<and> t = \<guillemotleft>t\<^sub>0\<guillemotright> \<and> \<not> wait\<^bold>} EvolveUntil \<delta> a \<sigma> ; T(C) \<^bold>{t \<le> \<guillemotleft>t\<^sub>0\<guillemotright> + \<guillemotleft>\<delta>\<guillemotright> \<longrightarrow> P \<and> \<guillemotleft>t\<^sub>0\<guillemotright> + \<guillemotleft>\<delta>\<guillemotright> \<le> t \<longrightarrow> R\<^bold>}"
+  apply (rule hoare_kcomp[where R="(P \<and> (\<not> wait \<longleftrightarrow> t = \<guillemotleft>t\<^sub>0\<guillemotright> + \<guillemotleft>\<delta>\<guillemotright>) \<and> (wait \<longleftrightarrow> t < \<guillemotleft>t\<^sub>0\<guillemotright> + \<guillemotleft>\<delta>\<guillemotright>))\<^sup>e"])
+  using assms apply (simp only:EvolveUntil_t_not_wait) (* Tentative *)
+  apply (rule hoare_T_wait) (* Need C to be monotonically increasing on t *)
+   defer
+  apply expr_auto
+  apply (rule hoare_weaken_pre_conj[where P="(P \<and> \<not> wait \<and> t = \<guillemotleft>t\<^sub>0\<guillemotright> + \<guillemotleft>\<delta>\<guillemotright> \<and> R)\<^sup>e"])
+  using assms apply expr_auto
+  apply (rule hoare_weaken_pre_conj[where P="(R)\<^sup>e"], expr_auto)
+  apply (rule hoare_stengthen_post[where Q="(R)\<^sup>e"])
+  using assms apply expr_auto
+  using assms by auto
+  
 lemma ini_cycle_loop:
   assumes "\<^bold>{P\<^bold>} I \<^bold>{P\<^bold>}" "\<^bold>{P\<^bold>} C \<^bold>{Q\<^bold>}" "\<^bold>{Q\<^bold>} C \<^bold>{Q\<^bold>}" "\<^bold>{Q\<^bold>} E \<^bold>{Q\<^bold>}"
   shows "\<^bold>{P\<^bold>} I ; C ; ((IF \<guillemotleft>TimeScale\<guillemotright>*\<guillemotleft>Cycle\<guillemotright> \<le> timer THEN C ELSE skip) ; E)\<^sup>* \<^bold>{Q\<^bold>}"
@@ -104,6 +353,26 @@ lemma cycle_loop':
 
 method hoare_cycle =
   (((simp only:kcomp_assoc)?, rule hoare_floyd_kcomp, subst_eval)+, subst_eval?, rule cycle_loop; hoare_help; hoare_help?)
+
+lemma cycle_loop'':
+  assumes "\<^bold>{P\<^bold>} C \<^bold>{R\<^bold>}" "\<^bold>{R\<^bold>} C \<^bold>{R\<^bold>}" "\<^bold>{R\<^bold>} E \<^bold>{R\<^bold>}"
+  shows "\<^bold>{P\<^bold>} (C ; E)\<^sup>* \<^bold>{R\<^bold>}"
+  oops (* TBC *)
+
+end
+
+term "[\<leadsto>] \<circ>\<^sub>s \<sigma>(x \<leadsto> u, x \<leadsto> v)"
+term "\<langle>\<sigma>(x \<leadsto> v, y \<leadsto> v)\<rangle>"
+term "\<langle>\<sigma>(x \<leadsto> v)\<rangle>"
+term "\<langle>CONST subst_upd [\<leadsto>] x (e)\<^sub>e\<rangle>"
+
+term "[\<leadsto>]"
+term "(subst_upd [\<leadsto>] x (e)\<^sub>e)"
+
+context robosim
+begin
+
+(* abbreviation (input) "TimerEvo \<delta> a \<sigma> B \<equiv> g_dl_ode_frame a \<sigma> (@B \<and> $timer \<le> \<delta>)\<^sub>e" *)
 
 end
 
